<?xml version="1.0"?>
<rdf:RDF
    xmlns:rdf="http://www.w3.org/1999/02/22-rdf-syntax-ns#"
    xmlns:rdfs="http://www.w3.org/2000/01/rdf-schema#"
    xmlns:pers-cat="https://data.gov.dk/concept/core/personaldata/"
    xmlns:dct="http://purl.org/dc/terms/"
    xmlns:dcat-dk="https://data.gov.dk/model/core/dcat-dk/"
    xmlns:conf="https://data.gov.dk/concept/core/confidentiality-type/"
    xmlns:adms="http://www.w3.org/ns/adms#"
    xmlns:mdl-app="https://data.gov.dk/concept/core/approvalstatus/"
    xmlns:owl="http://www.w3.org/2002/07/owl#"
    xmlns:skos="http://www.w3.org/2004/02/skos/core#"
    xmlns:dcat="http://www.w3.org/ns/dcat#"
    xmlns:org="http://www.w3.org/ns/org#"
    xmlns:vann="http://purl.org/vocab/vann/"
    xmlns:xsd="http://www.w3.org/2001/XMLSchema#"
  xml:base="https://data.gov.dk/model/core/dcat-dk">
  <owl:Ontology rdf:about="">
    <owl:versionInfo>version 1.0.0</owl:versionInfo>
    <mdl-app:approval rdf:resource="https://data.gov.dk/concept/core/approvalstatus/Approved"/>
    <rdfs:label xml:lang="da">DCAT vokabular udvidelse</rdfs:label>
    <rdfs:comment xml:lang="da">DCAT-DK er et vokabular, der udvider mulighederne for beskrivelse af datasæt i dansk fællesoffentlig kontekst og definerer egenskaber såsom datasætansvarlig, betalingspålagt, personoplysningskategori og fortrolighedsgrad, som ikke indgår i DCAT-AP eller DCAT.</rdfs:comment>
    <vann:preferredNamespacePrefix>dcat-dk</vann:preferredNamespacePrefix>
    <adms:status rdf:resource="http://purl.org/adms/status/Completed"/>
    <vann:preferredNamespaceUri>https://data.gov.dk/model/core/dcat-dk/</vann:preferredNamespaceUri>
    <dct:modified>2020-10-01</dct:modified>
    <rdfs:label xml:lang="en">DCAT vocabulary extension</rdfs:label>
    <owl:versionIRI rdf:resource="https://data.gov.dk/model/core/dcat-dk-1.0.0/"/>
    <dct:publisher>&lt;https://digst.dk/&gt;</dct:publisher>
    <rdfs:comment xml:lang="en">DCAT-DK is a vocabulary that expands the possibilities for describing data sets in the Danish common public context and defines characteristics such as data set manager, payment required, personal data category and degree of confidentiality, which are not included in DCAT-AP or DCAT.</rdfs:comment>
  </owl:Ontology>
  <owl:Class rdf:about="http://www.w3.org/ns/dcat#Dataset">
    <rdfs:isDefinedBy rdf:resource="http://www.w3.org/ns/dcat#"/>
    <rdfs:isDefinedBy rdf:resource="http://www.w3.org/TR/vocab-dcat/"/>
    <rdfs:comment xml:lang="da">En samling a data, udgivet eller organiseret af en enkelt kilde og som der er adgang til i en eller flere repræsentationer.</rdfs:comment>
    <rdfs:comment xml:lang="en">A collection of data, published or curated by a single source, and available for access or download in one or more represenations.</rdfs:comment>
    <rdfs:label xml:lang="da">Datasæt</rdfs:label>
    <rdfs:label xml:lang="en">Dataset</rdfs:label>
    <rdfs:subClassOf rdf:resource="http://www.w3.org/2002/07/owl#Thing"/>
  </owl:Class>
  <owl:Class rdf:about="https://data.gov.dk/concept/core/personaldata/PersonalDataCategory">
    <rdfs:label xml:lang="da">personoplysningskategori</rdfs:label>
    <rdfs:subClassOf rdf:resource="http://www.w3.org/2002/07/owl#Thing"/>
    <rdfs:label xml:lang="en">personal data category</rdfs:label>
    <rdfs:isDefinedBy rdf:resource="https://data.gov.dk/concept/core/personaldata/"/>
    <rdfs:comment xml:lang="en">classification according to the sensitivity of information as defifferent conditions and procedures for processing are applicable</rdfs:comment>
    <rdfs:comment xml:lang="da">kategori af personoplysninger set i forhold til følsomhed idet der gælder forskellige betingelser og procedurer for behandling af oplysningerne</rdfs:comment>
  </owl:Class>
  <owl:Class rdf:about="http://www.w3.org/ns/org#Organization">
    <rdfs:subClassOf rdf:resource="http://www.w3.org/2002/07/owl#Thing"/>
    <rdfs:isDefinedBy rdf:resource="http://www.w3.org/ns/org"/>
    <rdfs:comment xml:lang="en">Represents a collection of people organized together into a community or other social, commercial or political structure. The group has some common purpose or reason for existence which goes beyond the set of people belonging to it and can act as an Agent. Organizations are often decomposable into hierarchical structures.  It is recommended that SKOS lexical labels should be used to label the Organization. In particular `skos:prefLabel` for the primary (possibly legally recognized name), `skos:altLabel` for alternative names (trading names, colloquial names) and `skos:notation` to denote a code from a code list. Alternative names: _Collective_ _Body_ _Org_ _Group_</rdfs:comment>
    <rdfs:label xml:lang="en">Organization</rdfs:label>
    <rdfs:label xml:lang="da">Organisation</rdfs:label>
  </owl:Class>
  <owl:Class rdf:about="https://data.gov.dk/concept/core/confidentiality-type/ConfidentialityType">
    <rdfs:label xml:lang="da">fortrolighedsgrad</rdfs:label>
    <rdfs:label xml:lang="en">confidentiality degree</rdfs:label>
    <rdfs:comment xml:lang="en">degree of confidentiality with respect to the extent by which information can be disclosed</rdfs:comment>
    <rdfs:subClassOf rdf:resource="http://www.w3.org/2002/07/owl#Thing"/>
    <rdfs:comment xml:lang="da">grad af fortrolighed forstået som i hvilket omfang information kan videregives</rdfs:comment>
    <rdfs:isDefinedBy rdf:resource="https://data.gov.dk/concept/core/confidentiality-type/"/>
  </owl:Class>
  <owl:Class rdf:about="http://www.w3.org/ns/dcat#Resource">
    <rdfs:subClassOf rdf:resource="http://www.w3.org/2002/07/owl#Thing"/>
    <rdfs:label xml:lang="en">Catalogued resource</rdfs:label>
    <rdfs:label xml:lang="da">Katalogressource</rdfs:label>
    <rdfs:isDefinedBy rdf:resource="http://www.w3.org/TR/vocab-dcat/"/>
    <rdfs:isDefinedBy rdf:resource="http://www.w3.org/ns/dcat#"/>
  </owl:Class>
  <owl:ObjectProperty rdf:about="https://data.gov.dk/concept/core/approvalstatus/approval">
    <skos:prefLabel>approval</skos:prefLabel>
    <rdfs:label>approval</rdfs:label>
  </owl:ObjectProperty>
  <owl:ObjectProperty rdf:about="https://data.gov.dk/model/core/dcat-dk/datasetResponsibleOrganisation">
    <skos:definition xml:lang="en">organization that is legally accountable for the dataset</skos:definition>
    <rdfs:comment xml:lang="en">organization that is legally accountable for the dataset</rdfs:comment>
    <skos:definition xml:lang="da">organisation der har det juridiske ansvar for datasættet</skos:definition>
    <rdfs:label xml:lang="da">datasætansvarlig organisation</rdfs:label>
    <rdfs:comment xml:lang="da">organisation der har det juridiske ansvar for datasættet</rdfs:comment>
    <skos:prefLabel xml:lang="en">dataset responsible organisation</skos:prefLabel>
    <rdfs:domain rdf:resource="http://www.w3.org/ns/dcat#Dataset"/>
    <rdfs:label xml:lang="en">dataset responsible organisation</rdfs:label>
    <rdfs:range rdf:resource="http://www.w3.org/ns/org#Organization"/>
    <skos:prefLabel xml:lang="da">datasætansvarlig organisation</skos:prefLabel>
  </owl:ObjectProperty>
  <owl:ObjectProperty rdf:about="http://www.w3.org/ns/adms#status">
    <skos:prefLabel>status</skos:prefLabel>
    <rdfs:label>status</rdfs:label>
  </owl:ObjectProperty>
  <owl:ObjectProperty rdf:about="https://data.gov.dk/model/core/dcat-dk/hasConfidentialityType">
    <rdfs:isDefinedBy rdf:resource="https://data.gov.dk/model/core/dcat-dk/"/>
    <rdfs:label>has confidentiality type</rdfs:label>
    <rdfs:range rdf:resource="https://data.gov.dk/concept/core/confidentiality-type/ConfidentialityType"/>
    <skos:definition xml:lang="en">specification of the extent by which information can be disclosed</skos:definition>
    <skos:definition xml:lang="da">angivelse af i hvilket omfang information indeholdt i et datasæt kan videregives</skos:definition>
    <skos:prefLabel xml:lang="en">has confidentiality type</skos:prefLabel>
    <skos:prefLabel xml:lang="da">har fortrolighedsgrad</skos:prefLabel>
    <rdfs:domain rdf:resource="http://www.w3.org/ns/dcat#Dataset"/>
  </owl:ObjectProperty>
  <owl:ObjectProperty rdf:about="https://data.gov.dk/model/core/dcat-dk/personalDataCategory">
    <rdfs:label>personal data category</rdfs:label>
    <rdfs:domain rdf:resource="http://www.w3.org/ns/dcat#Dataset"/>
    <skos:definition xml:lang="da">angivelse af tilhørsforhold til en bestemt personoplysningskategori</skos:definition>
    <rdfs:comment xml:lang="en">Values for this property must be provided by a controlled vocabulary (A SKOS classification)</rdfs:comment>
    <skos:definition xml:lang="en">specification of a relation to specific personal data category</skos:definition>
    <skos:prefLabel xml:lang="en">personal data category</skos:prefLabel>
    <rdfs:comment xml:lang="da">Udfaldsrummet for denne egenskab skal være en klassifikation (SKOS)</rdfs:comment>
    <rdfs:isDefinedBy rdf:resource="https://data.gov.dk/model/core/dcat-dk/"/>
    <skos:prefLabel xml:lang="da">personoplysningskategori</skos:prefLabel>
    <rdfs:range rdf:resource="https://data.gov.dk/concept/core/personaldata/PersonalDataCategory"/>
  </owl:ObjectProperty>
  <rdf:Property rdf:about="http://purl.org/dc/terms/publisher">
    <skos:prefLabel>publisher</skos:prefLabel>
    <rdfs:label>publisher</rdfs:label>
  </rdf:Property>
  <owl:DatatypeProperty rdf:about="https://data.gov.dk/model/core/dcat-dk/paymentImposedContents">
    <rdfs:label xml:lang="en">payment imposed contents</rdfs:label>
    <rdfs:label xml:lang="da">betalingspålagt</rdfs:label>
    <skos:definition xml:lang="en">specification of whether payment is imposed on the catalogued resource or not.</skos:definition>
    <rdfs:range rdf:resource="http://www.w3.org/2001/XMLSchema#boolean"/>
    <skos:definition xml:lang="da">angivelse af hvorvidt datasættet er betalingspålagt eller ej.</skos:definition>
    <skos:prefLabel xml:lang="en">payment imposed contents</skos:prefLabel>
    <rdfs:domain rdf:resource="http://www.w3.org/ns/dcat#Resource"/>
    <skos:prefLabel xml:lang="da">betalingspålagt</skos:prefLabel>
    <rdfs:isDefinedBy rdf:resource="https://data.gov.dk/model/core/dcat-dk/"/>
  </owl:DatatypeProperty>
  <owl:DatatypeProperty rdf:about="http://www.w3.org/2004/02/skos/core#prefLabel">
    <rdfs:label>pref label</rdfs:label>
  </owl:DatatypeProperty>
  <owl:DatatypeProperty rdf:about="http://www.w3.org/2004/02/skos/core#altLabel">
    <rdfs:label>alt label</rdfs:label>
  </owl:DatatypeProperty>
  <owl:DatatypeProperty rdf:about="http://purl.org/vocab/vann/preferredNamespacePrefix">
    <rdfs:label>preferred namespace prefix</rdfs:label>
    <skos:prefLabel>preferred namespace prefix</skos:prefLabel>
  </owl:DatatypeProperty>
  <owl:DatatypeProperty rdf:about="http://www.w3.org/2004/02/skos/core#definition">
    <rdfs:label>definition</rdfs:label>
  </owl:DatatypeProperty>
  <owl:DatatypeProperty rdf:about="http://purl.org/vocab/vann/preferredNamespaceUri">
    <rdfs:label>preferred namespace uri</rdfs:label>
    <skos:prefLabel>preferred namespace uri</skos:prefLabel>
  </owl:DatatypeProperty>
  <owl:DatatypeProperty rdf:about="http://purl.org/dc/terms/modified">
    <skos:prefLabel>modified</skos:prefLabel>
    <rdfs:label>modified</rdfs:label>
  </owl:DatatypeProperty>
  <owl:DatatypeProperty rdf:about="http://www.w3.org/ns/dcat#theme">
    <dcat:theme>&lt;http://www.form-online.dk/opgavenoegle/06/#06.38.10.10&gt;</dcat:theme>
    <rdfs:label>theme</rdfs:label>
    <skos:prefLabel>theme</skos:prefLabel>
  </owl:DatatypeProperty>
</rdf:RDF>

<!-- Created with TopBraid -->
